

EQUATION SYSTEM FOR UNCONSTRAINED SAM MULTIPLIER

We replace actual numbers in the SAM with the following symbols.

	Activities		Commodities		Factors	House-holds	Exogenous demand	Total
	A1	A2	C1	C2	F	H	E	
A1			X ₁					X ₁
A2				X ₂				X ₂
C1	Z ₁₁	Z ₁₂				C ₁	E ₁	Z ₁
C2	Z ₂₁	Z ₂₂				C ₂	E ₂	Z ₂
F	V ₁	V ₂						V
H					V ₁ + V ₂			Y
E			L ₁	L ₂		S		E
Total	X ₁	X ₂	Z ₁	Z ₂	V	Y	E	

We divide columns by their total to derive the coefficients matrix (M-matrix). Note that the M-matrix excludes the exogenous components of demand.

	Activities		Commodities		Factors	House-holds	Exogenous demand	Total
	A1	A2	C1	C2	F	H	E	
A1			b ₁ = X ₁ /Z ₁					X ₁
A2				b ₂ = X ₂ /Z ₂				X ₂
C1	a ₁₁ = Z ₁₁ /X ₁	a ₁₂ = Z ₁₂ /X ₂				c ₁ = C ₁ /Y	E ₁	Z ₁
C2	a ₂₁ = Z ₂₁ /X ₁	a ₂₂ = Z ₂₂ /X ₂				c ₂ = C ₂ /Y	E ₂	Z ₂
F	v ₁ = V ₁ /X ₁	v ₂ = V ₂ /X ₂						V
H					1			Y
E			l ₁ = L ₁ /Z ₁	l ₂ = L ₂ /Z ₂		s = S/Y		E
Total	1	1	1	1	1	1	E	

Values

- X Gross output of each activity (i.e., X₁ and X₂)
- Z Total demand for each commodity (i.e., Z₁ and Z₂)
- V Total factor income (equal to household income)
- Y Total household income (equal to total factor income)
- E Exogenous components of demand (i.e., government, investment, and exports)

Shares

- a Technical coefficients (i.e., input or intermediate shares in production)
- b Share of domestic output in total demand
- v Share of value-added or factor income in gross output
- l Share of the value of total demand from imports or commodity taxes
- c Household consumption expenditure shares
- s Household savings rate (i.e., savings as a share of household income)

So we can now derive equations representing the relationships in the SAM. We start with the simple demand equations.

$$\begin{aligned} Z_1 &= a_{11}X_1 + a_{12}X_2 + c_1Y + E_1 \\ Z_2 &= a_{21}X_1 + a_{22}X_2 + c_2Y + E_2 \end{aligned} \quad (A1)$$

Total demand = intermediate demand + household demand + exogenous demand

From the SAM, we know that domestic production X is only part of total demand Z.

$$X_1 = b_1Z_1 \quad \text{and} \quad X_2 = b_2Z_2$$

We know that household income Y depends on the share each factor earns in each sector.

$$Y = v_1X_1 + v_2X_2 \quad \text{or} \quad Y = v_1b_1Z_1 + v_2b_2Z_2$$

Now we replace Xs and Vs in Equation A1.

$$\begin{aligned} Z_1 &= a_{11}b_1Z_1 + a_{12}b_2Z_2 + c_1(v_1b_1Z_1 + v_2b_2Z_2) + E_1 \\ Z_2 &= a_{21}b_1Z_1 + a_{22}b_2Z_2 + c_2(v_1b_1Z_1 + v_2b_2Z_2) + E_2 \end{aligned}$$

We move everything except for E onto the left-hand side.

$$\begin{aligned} Z_1 - a_{11}b_1Z_1 - c_1v_1b_1Z_1 - a_{12}b_2Z_2 - c_1v_2b_2Z_2 &= E_1 \\ -a_{21}b_1Z_1 - c_2v_1b_1Z_1 + Z_2 - a_{22}b_2Z_2 - c_2v_2b_2Z_2 &= E_2 \end{aligned}$$

We group Zs together.

$$\begin{aligned} (1 - a_{11}b_1 - c_1v_1b_1)Z_1 + (-a_{12}b_2 - c_1v_2b_2)Z_2 &= E_1 \\ (-a_{21}b_1 - c_2v_1b_1)Z_1 + (1 - a_{22}b_2 - c_2v_2b_2)Z_2 &= E_2 \end{aligned} \quad (A2)$$

We express Equation A2 in matrix format.

$$\begin{pmatrix} 1 - a_{11}b_1 - c_1v_1b_1 & -a_{12}b_2 - c_1v_2b_2 \\ -a_{21}b_1 - c_2v_1b_1 & 1 - a_{22}b_2 - c_2v_2b_2 \end{pmatrix} \begin{pmatrix} Z_1 \\ Z_2 \end{pmatrix} = \begin{pmatrix} E_1 \\ E_2 \end{pmatrix} \quad (A3)$$

The first term in Equation A3 is the identity matrix (I) minus the coefficient matrix (M).

$$\begin{pmatrix} 1 - a_{11}b_1 - c_1v_1b_1 & -a_{12}b_2 - c_1v_2b_2 \\ -a_{21}b_1 - c_2v_1b_1 & 1 - a_{22}b_2 - c_2v_2b_2 \end{pmatrix} = I - M$$

If we rename the other two vectors Z and E then we can simplify Equation A3.

$$(I - M)Z = E \quad (A4)$$

Rearranging, we get the final multiplier equation.

$$\begin{aligned} Z &= (I - M)^{-1}E \\ \text{Total demand} &= \text{multiplier matrix} \times \text{exogenous demand} \end{aligned} \quad (A5)$$

This tells us that when exogenous demand [E] increases, then after you have taken all the direct and indirect multiplier effects into account $[(I-M)^{-1}]$, you will end up with a final increase in total demand equal to Z.